<?xml version="1.0"?>
<rdf:RDF xmlns="http://purl.org/ontology/wsf#"
     xml:base="http://purl.org/ontology/wsf"
     xmlns:dc="http://purl.org/dc/elements/1.1/"
     xmlns:ns="http://www.w3.org/2003/06/sw-vocab-status/ns#"
     xmlns:foaf="http://xmlns.com/foaf/0.1/"
     xmlns:terms="http://purl.org/dc/terms/"
     xmlns:void="http://rdfs.org/ns/void#"
     xmlns:rdfs="http://www.w3.org/2000/01/rdf-schema#"
     xmlns:owl2xml="http://www.w3.org/2006/12/owl2-xml#"
     xmlns:xsd="http://www.w3.org/2001/XMLSchema#"
     xmlns:owl="http://www.w3.org/2002/07/owl#"
     xmlns:rdf="http://www.w3.org/1999/02/22-rdf-syntax-ns#"
     xmlns:doap="http://usefulinc.com/ns/doap#"
     xmlns:sco="http://purl.org/ontology/sco#">
    <owl:Ontology rdf:about="http://purl.org/ontology/wsf">
        <dc:title>Web Services Frameworks Ontology</dc:title>
        <dc:description xml:lang="en">An ontology for describing the structWSF web services frameworks instances.</dc:description>
        <owl:versionInfo>http://purl.org/ontology/wsf/0.1/</owl:versionInfo>
        <sco:ontologyType rdf:resource="http://purl.org/ontology/sco#administrativeOntology"/>
        <dc:creator rdf:resource="http://purl.org/ontology/wsf#fgiasson"/>
    </owl:Ontology>
    


    <!-- 
    ///////////////////////////////////////////////////////////////////////////////////////
    //
    // Annotation properties
    //
    ///////////////////////////////////////////////////////////////////////////////////////
     -->

    <owl:AnnotationProperty rdf:about="http://www.w3.org/2002/07/owl#versionInfo"/>
    <owl:AnnotationProperty rdf:about="http://purl.org/dc/elements/1.1/creator"/>
    <owl:AnnotationProperty rdf:about="http://www.w3.org/2000/01/rdf-schema#seeAlso"/>
    <owl:AnnotationProperty rdf:about="http://www.w3.org/2000/01/rdf-schema#isDefinedBy"/>
    <owl:AnnotationProperty rdf:about="http://www.w3.org/2003/06/sw-vocab-status/ns#term_status"/>
    <owl:AnnotationProperty rdf:about="http://www.w3.org/2000/01/rdf-schema#label"/>
    <owl:AnnotationProperty rdf:about="http://purl.org/dc/elements/1.1/description"/>
    <owl:AnnotationProperty rdf:about="http://purl.org/ontology/sco#ontologyType"/>
    <owl:AnnotationProperty rdf:about="http://www.w3.org/2000/01/rdf-schema#comment"/>
    <owl:AnnotationProperty rdf:about="http://purl.org/dc/elements/1.1/title"/>
    


    <!-- 
    ///////////////////////////////////////////////////////////////////////////////////////
    //
    // Datatypes
    //
    ///////////////////////////////////////////////////////////////////////////////////////
     -->

    


    <!-- 
    ///////////////////////////////////////////////////////////////////////////////////////
    //
    // Object Properties
    //
    ///////////////////////////////////////////////////////////////////////////////////////
     -->

    


    <!-- http://purl.org/ontology/wsf#datasetAccess -->

    <owl:ObjectProperty rdf:about="http://purl.org/ontology/wsf#datasetAccess">
        <rdfs:label xml:lang="en">dataset</rdfs:label>
        <rdfs:isDefinedBy rdf:datatype="http://www.w3.org/2001/XMLSchema#anyURI">http://purl.org/ontology/wsf#</rdfs:isDefinedBy>
        <rdfs:comment xml:lang="en">Links an Access instance to a dataset. This dataset belongs to the web services framework. </rdfs:comment>
        <rdfs:domain rdf:resource="http://purl.org/ontology/wsf#Access"/>
        <rdfs:range rdf:resource="http://rdfs.org/ns/void#Dataset"/>
    </owl:ObjectProperty>
    


    <!-- http://purl.org/ontology/wsf#fromDataset -->

    <owl:ObjectProperty rdf:about="http://purl.org/ontology/wsf#fromDataset">
        <rdfs:label xml:lang="en">from dataset</rdfs:label>
        <rdfs:isDefinedBy rdf:datatype="http://www.w3.org/2001/XMLSchema#anyURI">http://purl.org/ontology/wsf#</rdfs:isDefinedBy>
        <rdfs:comment xml:lang="en">Specifies the dataset provenance of the record that is related to the revision record.</rdfs:comment>
        <rdfs:domain rdf:resource="http://purl.org/ontology/wsf#Revision"/>
        <rdfs:range rdf:resource="http://rdfs.org/ns/void#Dataset"/>
    </owl:ObjectProperty>
    


    <!-- http://purl.org/ontology/wsf#hasAccess -->

    <owl:ObjectProperty rdf:about="http://purl.org/ontology/wsf#hasAccess">
        <rdfs:label xml:lang="en">has access</rdfs:label>
        <rdfs:isDefinedBy rdf:datatype="http://www.w3.org/2001/XMLSchema#anyURI">http://purl.org/ontology/wsf#</rdfs:isDefinedBy>
        <rdfs:comment xml:lang="en">Define an Access instance for a specific web service.</rdfs:comment>
        <rdfs:range rdf:resource="http://purl.org/ontology/wsf#Access"/>
        <rdfs:domain rdf:resource="http://purl.org/ontology/wsf#AuthenticationWebService"/>
    </owl:ObjectProperty>
    


    <!-- http://purl.org/ontology/wsf#hasAuthenticationWebService -->

    <owl:ObjectProperty rdf:about="http://purl.org/ontology/wsf#hasAuthenticationWebService">
        <rdfs:label xml:lang="en">has authentication web service</rdfs:label>
        <rdfs:isDefinedBy rdf:datatype="http://www.w3.org/2001/XMLSchema#anyURI">http://purl.org/ontology/wsf#</rdfs:isDefinedBy>
        <rdfs:comment xml:lang="en">Specifies what isthe web service, in the network, used for authentication purposes.</rdfs:comment>
        <rdfs:range rdf:resource="http://purl.org/ontology/wsf#AuthenticationWebService"/>
        <rdfs:domain rdf:resource="http://purl.org/ontology/wsf#WebServiceFramework"/>
        <rdfs:subPropertyOf rdf:resource="http://purl.org/ontology/wsf#hasWebService"/>
    </owl:ObjectProperty>
    


    <!-- http://purl.org/ontology/wsf#hasCrudUsage -->

    <owl:ObjectProperty rdf:about="http://purl.org/ontology/wsf#hasCrudUsage">
        <rdfs:label xml:lang="en">has access</rdfs:label>
        <rdfs:isDefinedBy rdf:datatype="http://www.w3.org/2001/XMLSchema#anyURI">http://purl.org/ontology/wsf#</rdfs:isDefinedBy>
        <rdfs:comment xml:lang="en">Define a CrudUsage instance for a specific web service.</rdfs:comment>
        <rdfs:range rdf:resource="http://purl.org/ontology/wsf#CrudUsage"/>
        <rdfs:domain rdf:resource="http://purl.org/ontology/wsf#WebService"/>
    </owl:ObjectProperty>
    


    <!-- http://purl.org/ontology/wsf#hasWebService -->

    <owl:ObjectProperty rdf:about="http://purl.org/ontology/wsf#hasWebService">
        <rdfs:label xml:lang="en">has web service</rdfs:label>
        <rdfs:isDefinedBy rdf:datatype="http://www.w3.org/2001/XMLSchema#anyURI">http://purl.org/ontology/wsf#</rdfs:isDefinedBy>
        <rdfs:comment xml:lang="en">Define the fact that a certain web service belong to a web service(s) framework.</rdfs:comment>
        <rdfs:range rdf:resource="http://purl.org/ontology/wsf#WebService"/>
        <rdfs:domain rdf:resource="http://purl.org/ontology/wsf#WebServiceFramework"/>
    </owl:ObjectProperty>
    


    <!-- http://purl.org/ontology/wsf#performer -->

    <owl:ObjectProperty rdf:about="http://purl.org/ontology/wsf#performer">
        <rdfs:label xml:lang="en">performer</rdfs:label>
        <rdfs:isDefinedBy rdf:datatype="http://www.w3.org/2001/XMLSchema#anyURI">http://purl.org/ontology/wsf#</rdfs:isDefinedBy>
        <rdfs:comment xml:lang="en">User that created the revision record.</rdfs:comment>
        <rdfs:domain rdf:resource="http://purl.org/ontology/wsf#Revision"/>
        <rdfs:range rdf:resource="http://xmlns.com/foaf/0.1/Agent"/>
    </owl:ObjectProperty>
    


    <!-- http://purl.org/ontology/wsf#revisionStatus -->

    <owl:ObjectProperty rdf:about="http://purl.org/ontology/wsf#revisionStatus">
        <rdfs:label xml:lang="en">revision status</rdfs:label>
        <rdfs:isDefinedBy rdf:datatype="http://www.w3.org/2001/XMLSchema#anyURI">http://purl.org/ontology/wsf#</rdfs:isDefinedBy>
        <rdfs:comment xml:lang="en">Specifies the current publication status of a revision record.</rdfs:comment>
        <rdfs:domain rdf:resource="http://purl.org/ontology/wsf#Revision"/>
        <rdfs:range rdf:resource="http://purl.org/ontology/wsf#RevisionStatus"/>
    </owl:ObjectProperty>
    


    <!-- http://purl.org/ontology/wsf#revisionUri -->

    <owl:ObjectProperty rdf:about="http://purl.org/ontology/wsf#revisionUri">
        <rdfs:label xml:lang="en">revision uri</rdfs:label>
        <rdfs:isDefinedBy rdf:datatype="http://www.w3.org/2001/XMLSchema#anyURI">http://purl.org/ontology/wsf#</rdfs:isDefinedBy>
        <rdfs:comment xml:lang="en">Link a revision record to the record it revisions.</rdfs:comment>
        <rdfs:domain rdf:resource="http://purl.org/ontology/wsf#Revision"/>
        <rdfs:range rdf:resource="http://www.w3.org/2002/07/owl#Thing"/>
    </owl:ObjectProperty>
    


    <!-- http://purl.org/ontology/wsf#webServiceAccess -->

    <owl:ObjectProperty rdf:about="http://purl.org/ontology/wsf#webServiceAccess">
        <rdfs:label xml:lang="en">dataset</rdfs:label>
        <rdfs:isDefinedBy rdf:datatype="http://www.w3.org/2001/XMLSchema#anyURI">http://purl.org/ontology/wsf#</rdfs:isDefinedBy>
        <rdfs:comment xml:lang="en">Links an Access instance to a web service. This web service belongs to the web services framework.</rdfs:comment>
        <rdfs:domain rdf:resource="http://purl.org/ontology/wsf#Access"/>
        <rdfs:range rdf:resource="http://purl.org/ontology/wsf#WebService"/>
    </owl:ObjectProperty>
    


    <!-- http://www.w3.org/2002/07/owl#topObjectProperty -->

    <owl:ObjectProperty rdf:about="http://www.w3.org/2002/07/owl#topObjectProperty"/>
    


    <!-- 
    ///////////////////////////////////////////////////////////////////////////////////////
    //
    // Data properties
    //
    ///////////////////////////////////////////////////////////////////////////////////////
     -->

    


    <!-- http://purl.org/ontology/wsf#collation -->

    <owl:DatatypeProperty rdf:about="http://purl.org/ontology/wsf#collation">
        <rdfs:label xml:lang="en">collation</rdfs:label>
        <rdfs:isDefinedBy rdf:datatype="http://www.w3.org/2001/XMLSchema#anyURI">http://purl.org/ontology/wsf#</rdfs:isDefinedBy>
        <rdfs:comment xml:lang="en">Specify the full corrected Search web service endpoint query that would have returned no results and that may have spelling issues.</rdfs:comment>
        <rdfs:domain rdf:resource="http://purl.org/ontology/wsf#SpellSuggestion"/>
    </owl:DatatypeProperty>
    


    <!-- http://purl.org/ontology/wsf#create -->

    <owl:DatatypeProperty rdf:about="http://purl.org/ontology/wsf#create">
        <rdfs:label xml:lang="en">create access</rdfs:label>
        <rdfs:isDefinedBy rdf:datatype="http://www.w3.org/2001/XMLSchema#anyURI">http://purl.org/ontology/wsf#</rdfs:isDefinedBy>
        <rdfs:comment xml:lang="en">The create access function is used to specify if a certain IP (part of an Access instance) has create access to the web service(s) framework.</rdfs:comment>
        <rdfs:domain rdf:resource="http://purl.org/ontology/wsf#Access"/>
        <rdfs:subPropertyOf rdf:resource="http://purl.org/ontology/wsf#usageFunction"/>
        <rdfs:range rdf:resource="http://www.w3.org/2001/XMLSchema#boolean"/>
    </owl:DatatypeProperty>
    


    <!-- http://purl.org/ontology/wsf#crudAction -->

    <owl:DatatypeProperty rdf:about="http://purl.org/ontology/wsf#crudAction">
        <rdfs:label xml:lang="en">crud action</rdfs:label>
        <rdfs:isDefinedBy rdf:datatype="http://www.w3.org/2001/XMLSchema#anyURI">http://purl.org/ontology/wsf#</rdfs:isDefinedBy>
        <rdfs:comment xml:lang="en">States the CRUD action that should be used to index a given record into structWSF. This property is used by the Datasets Syncing Framework to determine if the record feed to it should be created, deleted or updated.

The value of this property can be one of:

(1) create
(2) update
(3) delete

This property is used by the Datasets Syncing Framework.</rdfs:comment>
    </owl:DatatypeProperty>
    


    <!-- http://purl.org/ontology/wsf#delete -->

    <owl:DatatypeProperty rdf:about="http://purl.org/ontology/wsf#delete">
        <rdfs:label xml:lang="en">delete access</rdfs:label>
        <rdfs:isDefinedBy rdf:datatype="http://www.w3.org/2001/XMLSchema#anyURI">http://purl.org/ontology/wsf#</rdfs:isDefinedBy>
        <rdfs:comment xml:lang="en">The delete access function is used to specify if a certain IP (part of an Access instance) has delete access to the web service(s) framework.</rdfs:comment>
        <rdfs:domain rdf:resource="http://purl.org/ontology/wsf#Access"/>
        <rdfs:subPropertyOf rdf:resource="http://purl.org/ontology/wsf#usageFunction"/>
        <rdfs:range rdf:resource="http://www.w3.org/2001/XMLSchema#boolean"/>
    </owl:DatatypeProperty>
    


    <!-- http://purl.org/ontology/wsf#endpoint -->

    <owl:DatatypeProperty rdf:about="http://purl.org/ontology/wsf#endpoint">
        <rdfs:label xml:lang="en">endpoint</rdfs:label>
        <rdfs:isDefinedBy rdf:datatype="http://www.w3.org/2001/XMLSchema#anyURI">http://purl.org/ontology/wsf#</rdfs:isDefinedBy>
        <rdfs:comment xml:lang="en">URL of the endpoint where wecan have access to the web service on the Web.</rdfs:comment>
        <rdfs:domain rdf:resource="http://purl.org/ontology/wsf#WebService"/>
        <rdfs:range rdf:resource="http://www.w3.org/2000/01/rdf-schema#Literal"/>
    </owl:DatatypeProperty>
    


    <!-- http://purl.org/ontology/wsf#frequency -->

    <owl:DatatypeProperty rdf:about="http://purl.org/ontology/wsf#frequency">
        <rdfs:label xml:lang="en">frequency</rdfs:label>
        <rdfs:isDefinedBy rdf:datatype="http://www.w3.org/2001/XMLSchema#anyURI">http://purl.org/ontology/wsf#</rdfs:isDefinedBy>
        <rdfs:comment xml:lang="en">Specify frequency of a suggested term to correct a missspelled word used within a Search web service query. This frequency can be used to order all the suggest terms for a misspelled keyword.</rdfs:comment>
        <rdfs:domain rdf:resource="http://purl.org/ontology/wsf#SpellSuggestion"/>
    </owl:DatatypeProperty>
    


    <!-- http://purl.org/ontology/wsf#holdOntology -->

    <owl:DatatypeProperty rdf:about="http://purl.org/ontology/wsf#holdOntology">
        <rdfs:label xml:lang="en">hold ontology</rdfs:label>
        <rdfs:isDefinedBy rdf:datatype="http://www.w3.org/2001/XMLSchema#anyURI">http://purl.org/ontology/wsf#</rdfs:isDefinedBy>
        <rdfs:comment xml:lang="en">Specifies that a dataset hold an ontology description.</rdfs:comment>
        <rdfs:domain rdf:resource="http://rdfs.org/ns/void#Dataset"/>
        <rdfs:range rdf:resource="http://www.w3.org/2000/01/rdf-schema#Literal"/>
    </owl:DatatypeProperty>
    


    <!-- http://purl.org/ontology/wsf#objectLabel -->

    <owl:DatatypeProperty rdf:about="http://purl.org/ontology/wsf#objectLabel">
        <rdfs:label xml:lang="en">object label</rdfs:label>
        <rdfs:isDefinedBy rdf:datatype="http://www.w3.org/2001/XMLSchema#anyURI">http://purl.org/ontology/wsf#</rdfs:isDefinedBy>
        <rdfs:comment xml:lang="en">Used to specify the label of a record referenced by an object property.

This properly is used to reify the label of a referenced object record in an object property triple.</rdfs:comment>
    </owl:DatatypeProperty>
    


    <!-- http://purl.org/ontology/wsf#ontologyModified -->

    <owl:DatatypeProperty rdf:about="http://purl.org/ontology/wsf#ontologyModified">
        <rdfs:label xml:lang="en">ontology modified</rdfs:label>
        <rdfs:isDefinedBy rdf:datatype="http://www.w3.org/2001/XMLSchema#anyURI">http://purl.org/ontology/wsf#</rdfs:isDefinedBy>
        <rdfs:comment xml:lang="en">States if an ontology has been modified since the last time it got saved on the file system of the OSF server instance.

This is used by the structOntology conStruct module.</rdfs:comment>
        <rdfs:domain rdf:resource="http://rdfs.org/ns/void#Dataset"/>
        <rdfs:range rdf:resource="http://www.w3.org/2001/XMLSchema#boolean"/>
    </owl:DatatypeProperty>
    


    <!-- http://purl.org/ontology/wsf#read -->

    <owl:DatatypeProperty rdf:about="http://purl.org/ontology/wsf#read">
        <rdfs:label xml:lang="en">read access</rdfs:label>
        <rdfs:isDefinedBy rdf:datatype="http://www.w3.org/2001/XMLSchema#anyURI">http://purl.org/ontology/wsf#</rdfs:isDefinedBy>
        <rdfs:comment xml:lang="en">The read access function is used to specify if a certain IP (part of an Access instance) has read access to the web service(s) framework.</rdfs:comment>
        <rdfs:domain rdf:resource="http://purl.org/ontology/wsf#Access"/>
        <rdfs:subPropertyOf rdf:resource="http://purl.org/ontology/wsf#usageFunction"/>
        <rdfs:range rdf:resource="http://www.w3.org/2001/XMLSchema#boolean"/>
    </owl:DatatypeProperty>
    


    <!-- http://purl.org/ontology/wsf#registeredIP -->

    <owl:DatatypeProperty rdf:about="http://purl.org/ontology/wsf#registeredIP">
        <rdfs:label xml:lang="en">registered IP address</rdfs:label>
        <rdfs:isDefinedBy rdf:datatype="http://www.w3.org/2001/XMLSchema#anyURI">http://purl.org/ontology/wsf#</rdfs:isDefinedBy>
        <rdfs:comment xml:lang="en">An IP address that is registered to a web service. This means that requests from that IP address can be answered by the web service endpoint given its CRUD permissions.

This is the first authentication/encryption layer of the web service security stack.</rdfs:comment>
        <rdfs:domain rdf:resource="http://purl.org/ontology/wsf#Access"/>
        <rdfs:range rdf:resource="http://www.w3.org/2000/01/rdf-schema#Literal"/>
    </owl:DatatypeProperty>
    


    <!-- http://purl.org/ontology/wsf#revisionTime -->

    <owl:DatatypeProperty rdf:about="http://purl.org/ontology/wsf#revisionTime">
        <rdfs:label xml:lang="en">revision time</rdfs:label>
        <rdfs:isDefinedBy rdf:datatype="http://www.w3.org/2001/XMLSchema#anyURI">http://purl.org/ontology/wsf#</rdfs:isDefinedBy>
        <rdfs:comment xml:lang="en">This is the Unix time stamp (which includes microseconds) when the revision got created

The sequence of revisions is determined by the time when they got created. The correct sequence of revisions of a record can be re-created by ordering them by these time stamps.

The value of this property is filled at creation time of the revision.</rdfs:comment>
        <rdfs:domain rdf:resource="http://purl.org/ontology/wsf#Revision"/>
        <rdfs:range rdf:resource="http://www.w3.org/2000/01/rdf-schema#Literal"/>
    </owl:DatatypeProperty>
    


    <!-- http://purl.org/ontology/wsf#suggestion -->

    <owl:DatatypeProperty rdf:about="http://purl.org/ontology/wsf#suggestion">
        <rdfs:label xml:lang="en">suggestion</rdfs:label>
        <rdfs:isDefinedBy rdf:datatype="http://www.w3.org/2001/XMLSchema#anyURI">http://purl.org/ontology/wsf#</rdfs:isDefinedBy>
        <rdfs:comment xml:lang="en">Specify a suggested term to correct a missspelled word used within a Search web service query.</rdfs:comment>
        <rdfs:domain rdf:resource="http://purl.org/ontology/wsf#SpellSuggestion"/>
    </owl:DatatypeProperty>
    


    <!-- http://purl.org/ontology/wsf#update -->

    <owl:DatatypeProperty rdf:about="http://purl.org/ontology/wsf#update">
        <rdfs:label xml:lang="en">update access</rdfs:label>
        <rdfs:isDefinedBy rdf:datatype="http://www.w3.org/2001/XMLSchema#anyURI">http://purl.org/ontology/wsf#</rdfs:isDefinedBy>
        <rdfs:comment xml:lang="en">The update access function is used to specify if a certain IP (part of an Access instance) has update access to the web service(s) framework.</rdfs:comment>
        <rdfs:domain rdf:resource="http://purl.org/ontology/wsf#Access"/>
        <rdfs:subPropertyOf rdf:resource="http://purl.org/ontology/wsf#usageFunction"/>
        <rdfs:range rdf:resource="http://www.w3.org/2001/XMLSchema#boolean"/>
    </owl:DatatypeProperty>
    


    <!-- http://purl.org/ontology/wsf#usageFunction -->

    <owl:DatatypeProperty rdf:about="http://purl.org/ontology/wsf#usageFunction">
        <rdfs:label xml:lang="en">usage function</rdfs:label>
        <rdfs:isDefinedBy rdf:datatype="http://www.w3.org/2001/XMLSchema#anyURI">http://purl.org/ontology/wsf#</rdfs:isDefinedBy>
        <rdfs:comment xml:lang="en">General usage function definition. These functions are used to specify if a certain IP (part of an Access instance) has some access to the web service(s) framework.</rdfs:comment>
        <rdfs:domain rdf:resource="http://purl.org/ontology/wsf#Access"/>
        <rdfs:range rdf:resource="http://www.w3.org/2001/XMLSchema#boolean"/>
    </owl:DatatypeProperty>
    


    <!-- http://www.w3.org/2002/07/owl#topDataProperty -->

    <owl:DatatypeProperty rdf:about="http://www.w3.org/2002/07/owl#topDataProperty"/>
    


    <!-- 
    ///////////////////////////////////////////////////////////////////////////////////////
    //
    // Classes
    //
    ///////////////////////////////////////////////////////////////////////////////////////
     -->

    


    <!-- http://purl.org/ontology/wsf#Access -->

    <owl:Class rdf:about="http://purl.org/ontology/wsf#Access">
        <rdfs:label xml:lang="en">Set of permissions</rdfs:label>
        <rdfs:subClassOf rdf:resource="http://www.w3.org/2002/07/owl#Thing"/>
        <rdfs:subClassOf>
            <owl:Restriction>
                <owl:onProperty rdf:resource="http://purl.org/ontology/wsf#update"/>
                <owl:cardinality rdf:datatype="http://www.w3.org/2001/XMLSchema#nonNegativeInteger">1</owl:cardinality>
            </owl:Restriction>
        </rdfs:subClassOf>
        <rdfs:subClassOf>
            <owl:Restriction>
                <owl:onProperty rdf:resource="http://purl.org/ontology/wsf#datasetAccess"/>
                <owl:onClass rdf:resource="http://rdfs.org/ns/void#Dataset"/>
                <owl:qualifiedCardinality rdf:datatype="http://www.w3.org/2001/XMLSchema#nonNegativeInteger">1</owl:qualifiedCardinality>
            </owl:Restriction>
        </rdfs:subClassOf>
        <rdfs:subClassOf>
            <owl:Restriction>
                <owl:onProperty rdf:resource="http://purl.org/ontology/wsf#create"/>
                <owl:cardinality rdf:datatype="http://www.w3.org/2001/XMLSchema#nonNegativeInteger">1</owl:cardinality>
            </owl:Restriction>
        </rdfs:subClassOf>
        <rdfs:subClassOf>
            <owl:Restriction>
                <owl:onProperty rdf:resource="http://purl.org/ontology/wsf#webServiceAccess"/>
                <owl:someValuesFrom rdf:resource="http://purl.org/ontology/wsf#WebService"/>
            </owl:Restriction>
        </rdfs:subClassOf>
        <rdfs:subClassOf>
            <owl:Restriction>
                <owl:onProperty rdf:resource="http://purl.org/ontology/wsf#delete"/>
                <owl:cardinality rdf:datatype="http://www.w3.org/2001/XMLSchema#nonNegativeInteger">1</owl:cardinality>
            </owl:Restriction>
        </rdfs:subClassOf>
        <rdfs:subClassOf>
            <owl:Restriction>
                <owl:onProperty rdf:resource="http://purl.org/ontology/wsf#read"/>
                <owl:cardinality rdf:datatype="http://www.w3.org/2001/XMLSchema#nonNegativeInteger">1</owl:cardinality>
            </owl:Restriction>
        </rdfs:subClassOf>
        <rdfs:isDefinedBy rdf:datatype="http://www.w3.org/2001/XMLSchema#anyURI">http://purl.org/ontology/wsf#</rdfs:isDefinedBy>
        <rdfs:comment xml:lang="en">A set of permissions to access a web services framework.

A set of permissions is defined by the four basic operations that can be performed on any web service: (1) create, (2) read, (3) update and (4) delete; ; it is defined by a IP address that has access to the web services endpoints and a specific dataset belonging to the web services framework.</rdfs:comment>
    </owl:Class>
    


    <!-- http://purl.org/ontology/wsf#AuthenticationWebService -->

    <owl:Class rdf:about="http://purl.org/ontology/wsf#AuthenticationWebService">
        <rdfs:label xml:lang="en">Authentication web service</rdfs:label>
        <rdfs:subClassOf rdf:resource="http://purl.org/ontology/wsf#WebService"/>
        <rdfs:subClassOf>
            <owl:Restriction>
                <owl:onProperty rdf:resource="http://purl.org/ontology/wsf#hasAccess"/>
                <owl:onClass rdf:resource="http://purl.org/ontology/wsf#Access"/>
                <owl:minQualifiedCardinality rdf:datatype="http://www.w3.org/2001/XMLSchema#nonNegativeInteger">1</owl:minQualifiedCardinality>
            </owl:Restriction>
        </rdfs:subClassOf>
        <rdfs:isDefinedBy rdf:datatype="http://www.w3.org/2001/XMLSchema#anyURI">http://purl.org/ontology/wsf#</rdfs:isDefinedBy>
        <rdfs:comment xml:lang="en">The authentication web service of a framework is a necessary web service that handle the authentication of users, permissions of access and registration of web services.</rdfs:comment>
    </owl:Class>
    


    <!-- http://purl.org/ontology/wsf#CrudUsage -->

    <owl:Class rdf:about="http://purl.org/ontology/wsf#CrudUsage">
        <rdfs:label xml:lang="en">Set of permissions</rdfs:label>
        <rdfs:subClassOf rdf:resource="http://www.w3.org/2002/07/owl#Thing"/>
        <rdfs:subClassOf>
            <owl:Restriction>
                <owl:onProperty rdf:resource="http://purl.org/ontology/wsf#update"/>
                <owl:cardinality rdf:datatype="http://www.w3.org/2001/XMLSchema#nonNegativeInteger">1</owl:cardinality>
            </owl:Restriction>
        </rdfs:subClassOf>
        <rdfs:subClassOf>
            <owl:Restriction>
                <owl:onProperty rdf:resource="http://purl.org/ontology/wsf#delete"/>
                <owl:cardinality rdf:datatype="http://www.w3.org/2001/XMLSchema#nonNegativeInteger">1</owl:cardinality>
            </owl:Restriction>
        </rdfs:subClassOf>
        <rdfs:subClassOf>
            <owl:Restriction>
                <owl:onProperty rdf:resource="http://purl.org/ontology/wsf#read"/>
                <owl:cardinality rdf:datatype="http://www.w3.org/2001/XMLSchema#nonNegativeInteger">1</owl:cardinality>
            </owl:Restriction>
        </rdfs:subClassOf>
        <rdfs:subClassOf>
            <owl:Restriction>
                <owl:onProperty rdf:resource="http://purl.org/ontology/wsf#create"/>
                <owl:cardinality rdf:datatype="http://www.w3.org/2001/XMLSchema#nonNegativeInteger">1</owl:cardinality>
            </owl:Restriction>
        </rdfs:subClassOf>
        <rdfs:isDefinedBy rdf:datatype="http://www.w3.org/2001/XMLSchema#anyURI">http://purl.org/ontology/wsf#</rdfs:isDefinedBy>
        <rdfs:comment xml:lang="en">A set of usage function that are performed by the web service

Any web service can do one, or many of these 4 basic usage function: (1) create, (2) read, (3) update and (4) delete. A CrudUsage instance define which of the 4 basic operations are performed by this specific web service. This information is then used with the Access permissions of a requester to find out if the request can be processed, or not, by the web service.</rdfs:comment>
    </owl:Class>
    


    <!-- http://purl.org/ontology/wsf#Revision -->

    <owl:Class rdf:about="http://purl.org/ontology/wsf#Revision">
        <rdfs:label xml:lang="en">revision</rdfs:label>
        <rdfs:isDefinedBy rdf:datatype="http://www.w3.org/2001/XMLSchema#anyURI">http://purl.org/ontology/wsf#</rdfs:isDefinedBy>
        <rdfs:comment xml:lang="en">A revision or a record indexed in a structWSF dataset. This revision record is used to &apos;save&apos; the state of a record after an update query.</rdfs:comment>
    </owl:Class>
    


    <!-- http://purl.org/ontology/wsf#RevisionStatus -->

    <owl:Class rdf:about="http://purl.org/ontology/wsf#RevisionStatus">
        <rdfs:label xml:lang="en">revision status</rdfs:label>
        <rdfs:isDefinedBy rdf:datatype="http://www.w3.org/2001/XMLSchema#anyURI">http://purl.org/ontology/wsf#</rdfs:isDefinedBy>
        <rdfs:comment xml:lang="en">A set of status that can be related to a revision record. This is what tells the users if a revision record is currently published, or what is the status of the revision in a publication workflow.</rdfs:comment>
    </owl:Class>
    


    <!-- http://purl.org/ontology/wsf#SpellSuggestion -->

    <owl:Class rdf:about="http://purl.org/ontology/wsf#SpellSuggestion">
        <rdfs:label xml:lang="en">Spell suggestion</rdfs:label>
        <rdfs:isDefinedBy rdf:datatype="http://www.w3.org/2001/XMLSchema#anyURI">http://purl.org/ontology/wsf#</rdfs:isDefinedBy>
        <rdfs:comment xml:lang="en">Used by the structWSF Search web service endpoint to define spell suggestions if a search query returns no result and if the spellcheck parameter is true.</rdfs:comment>
    </owl:Class>
    


    <!-- http://purl.org/ontology/wsf#WebService -->

    <owl:Class rdf:about="http://purl.org/ontology/wsf#WebService">
        <rdfs:label xml:lang="en">Web service</rdfs:label>
        <rdfs:subClassOf rdf:resource="http://www.w3.org/2002/07/owl#Thing"/>
        <rdfs:subClassOf>
            <owl:Restriction>
                <owl:onProperty rdf:resource="http://purl.org/ontology/wsf#endpoint"/>
                <owl:minCardinality rdf:datatype="http://www.w3.org/2001/XMLSchema#nonNegativeInteger">1</owl:minCardinality>
            </owl:Restriction>
        </rdfs:subClassOf>
        <rdfs:subClassOf>
            <owl:Restriction>
                <owl:onProperty rdf:resource="http://purl.org/ontology/wsf#hasCrudUsage"/>
                <owl:onClass rdf:resource="http://purl.org/ontology/wsf#CrudUsage"/>
                <owl:qualifiedCardinality rdf:datatype="http://www.w3.org/2001/XMLSchema#nonNegativeInteger">1</owl:qualifiedCardinality>
            </owl:Restriction>
        </rdfs:subClassOf>
        <rdfs:isDefinedBy rdf:datatype="http://www.w3.org/2001/XMLSchema#anyURI">http://purl.org/ontology/wsf#</rdfs:isDefinedBy>
        <rdfs:comment xml:lang="en">A web service</rdfs:comment>
    </owl:Class>
    


    <!-- http://purl.org/ontology/wsf#WebServiceFramework -->

    <owl:Class rdf:about="http://purl.org/ontology/wsf#WebServiceFramework">
        <rdfs:label xml:lang="en">Web service(s) framework</rdfs:label>
        <rdfs:subClassOf rdf:resource="http://www.w3.org/2002/07/owl#Thing"/>
        <rdfs:subClassOf>
            <owl:Restriction>
                <owl:onProperty rdf:resource="http://purl.org/ontology/wsf#hasAuthenticationWebService"/>
                <owl:onClass rdf:resource="http://purl.org/ontology/wsf#AuthenticationWebService"/>
                <owl:qualifiedCardinality rdf:datatype="http://www.w3.org/2001/XMLSchema#nonNegativeInteger">1</owl:qualifiedCardinality>
            </owl:Restriction>
        </rdfs:subClassOf>
        <rdfs:isDefinedBy rdf:datatype="http://www.w3.org/2001/XMLSchema#anyURI">http://purl.org/ontology/wsf#</rdfs:isDefinedBy>
        <rdfs:comment xml:lang="en">A framework of web services</rdfs:comment>
    </owl:Class>
    


    <!-- http://rdfs.org/ns/void#Dataset -->

    <owl:Class rdf:about="http://rdfs.org/ns/void#Dataset"/>
    


    <!-- http://www.w3.org/2002/07/owl#Thing -->

    <owl:Class rdf:about="http://www.w3.org/2002/07/owl#Thing"/>
    


    <!-- http://xmlns.com/foaf/0.1/Agent -->

    <owl:Class rdf:about="http://xmlns.com/foaf/0.1/Agent"/>
    


    <!-- http://xmlns.com/foaf/0.1/Person -->

    <owl:Class rdf:about="http://xmlns.com/foaf/0.1/Person">
        <rdfs:subClassOf rdf:resource="http://xmlns.com/foaf/0.1/Agent"/>
    </owl:Class>
    


    <!-- 
    ///////////////////////////////////////////////////////////////////////////////////////
    //
    // Individuals
    //
    ///////////////////////////////////////////////////////////////////////////////////////
     -->

    


    <!-- http://purl.org/ontology/wsf#archive -->

    <owl:NamedIndividual rdf:about="http://purl.org/ontology/wsf#archive">
        <rdf:type rdf:resource="http://purl.org/ontology/wsf#RevisionStatus"/>
        <rdfs:label xml:lang="en">archive</rdfs:label>
        <rdfs:isDefinedBy rdf:datatype="http://www.w3.org/2001/XMLSchema#anyURI">http://purl.org/ontology/wsf#</rdfs:isDefinedBy>
    </owl:NamedIndividual>
    


    <!-- http://purl.org/ontology/wsf#experimental -->

    <owl:NamedIndividual rdf:about="http://purl.org/ontology/wsf#experimental">
        <rdf:type rdf:resource="http://purl.org/ontology/wsf#RevisionStatus"/>
        <rdfs:label xml:lang="en">experimental</rdfs:label>
        <rdfs:isDefinedBy rdf:datatype="http://www.w3.org/2001/XMLSchema#anyURI">http://purl.org/ontology/wsf#</rdfs:isDefinedBy>
    </owl:NamedIndividual>
    


    <!-- http://purl.org/ontology/wsf#fgiasson -->

    <owl:NamedIndividual rdf:about="http://purl.org/ontology/wsf#fgiasson">
        <rdf:type rdf:resource="http://xmlns.com/foaf/0.1/Person"/>
        <rdfs:seeAlso rdf:datatype="http://www.w3.org/2001/XMLSchema#anyURI">http://fgiasson.com/</rdfs:seeAlso>
        <rdfs:isDefinedBy rdf:datatype="http://www.w3.org/2001/XMLSchema#anyURI">http://purl.org/ontology/wsf#</rdfs:isDefinedBy>
    </owl:NamedIndividual>
    


    <!-- http://purl.org/ontology/wsf#harvesting -->

    <owl:NamedIndividual rdf:about="http://purl.org/ontology/wsf#harvesting">
        <rdf:type rdf:resource="http://purl.org/ontology/wsf#RevisionStatus"/>
        <rdfs:label xml:lang="en">harvesting</rdfs:label>
        <rdfs:isDefinedBy rdf:datatype="http://www.w3.org/2001/XMLSchema#anyURI">http://purl.org/ontology/wsf#</rdfs:isDefinedBy>
    </owl:NamedIndividual>
    


    <!-- http://purl.org/ontology/wsf#pre_release -->

    <owl:NamedIndividual rdf:about="http://purl.org/ontology/wsf#pre_release">
        <rdf:type rdf:resource="http://purl.org/ontology/wsf#RevisionStatus"/>
        <rdfs:label xml:lang="en">pre-release</rdfs:label>
        <rdfs:isDefinedBy rdf:datatype="http://www.w3.org/2001/XMLSchema#anyURI">http://purl.org/ontology/wsf#</rdfs:isDefinedBy>
    </owl:NamedIndividual>
    


    <!-- http://purl.org/ontology/wsf#published -->

    <owl:NamedIndividual rdf:about="http://purl.org/ontology/wsf#published">
        <rdf:type rdf:resource="http://purl.org/ontology/wsf#RevisionStatus"/>
        <rdfs:label xml:lang="en">published</rdfs:label>
        <rdfs:isDefinedBy rdf:datatype="http://www.w3.org/2001/XMLSchema#anyURI">http://purl.org/ontology/wsf#</rdfs:isDefinedBy>
    </owl:NamedIndividual>
    


    <!-- http://purl.org/ontology/wsf#staging -->

    <owl:NamedIndividual rdf:about="http://purl.org/ontology/wsf#staging">
        <rdf:type rdf:resource="http://purl.org/ontology/wsf#RevisionStatus"/>
        <rdfs:label xml:lang="en">staging</rdfs:label>
        <rdfs:isDefinedBy rdf:datatype="http://www.w3.org/2001/XMLSchema#anyURI">http://purl.org/ontology/wsf#</rdfs:isDefinedBy>
    </owl:NamedIndividual>
    


    <!-- http://purl.org/ontology/wsf#unspecified -->

    <owl:NamedIndividual rdf:about="http://purl.org/ontology/wsf#unspecified">
        <rdf:type rdf:resource="http://purl.org/ontology/wsf#RevisionStatus"/>
        <rdfs:label xml:lang="en">unspecified</rdfs:label>
        <rdfs:isDefinedBy rdf:datatype="http://www.w3.org/2001/XMLSchema#anyURI">http://purl.org/ontology/wsf#</rdfs:isDefinedBy>
    </owl:NamedIndividual>
</rdf:RDF>



<!-- Generated by the OWL API (version 3.3.1957) http://owlapi.sourceforge.net -->

